Makefile
@@ -1,12 +1,15 @@
 JXL_HOME ?= ../jxl-rs
 
-all: extract
+all: prove
 
 .PHONY: jxl.llbc
 jxl.llbc:
-	# FIXME: $(PWD) will not work if this MAkefile is invoked with make -C 
+	# FIXME: $(PWD) will not work if this Makefile is invoked with make -C 
 	../charon/bin/charon cargo --preset=aeneas --start-from="jxl::entropy_coding::ans::_::read" -- -p jxl --manifest-path $(JXL_HOME)/Cargo.toml
 	mv $(JXL_HOME)/$@ $@
 
 extract: jxl.llbc
-	cd lean && ../aeneas/bin/aeneas ../jxl.llbc -backend lean -split-files -subdir JxlProofs
+	../aeneas/bin/aeneas $< -backend lean -split-files -dest lean -subdir JxlProofs
+
+prove: extract
+	cd lean && lake build
